Make context support notation-only

ContextBasicDenotation/theories/RelevantEnv.v
@@ -18,20 +18,21 @@ Local Notation "m ⊨ φ" := (res_models m φ)
 Definition lty_env_restrict_lvars (Σ : lty_env) (D : lvset) : lty_env :=
   storeA_restrict Σ D.
 
-Definition context_tm_support (τ : context_ty) (e : tm) : lvset :=
-  context_ty_lvars τ ∪ tm_lvars e.
+Notation "'context_tm_support' τ e" :=
+  (context_ty_lvars τ ∪ tm_lvars e)
+  (at level 10, τ at next level, e at next level, only parsing).
 
 Definition relevant_lvars (τ : context_ty) (e : tm) : lvset :=
-  context_tm_support τ e.
+  context_ty_lvars τ ∪ tm_lvars e.
 
 Definition relevant_env (Σ : lty_env) (τ : context_ty) (e : tm)
     : lty_env :=
-  lty_env_restrict_lvars Σ (context_tm_support τ e).
+  lty_env_restrict_lvars Σ (context_ty_lvars τ ∪ tm_lvars e).
 
 Lemma lvars_fv_context_tm_support τ e :
-  lvars_fv (context_tm_support τ e) = fv_cty τ ∪ fv_tm e.
+  lvars_fv (context_ty_lvars τ ∪ tm_lvars e) = fv_cty τ ∪ fv_tm e.
 Proof.
-  unfold context_tm_support.
+  cbn [context_ty_lvars context_ty_lvars_at tm_lvars tm_lvars_at value_lvars value_lvars_at].
   rewrite lvars_fv_union, context_ty_lvars_fv, tm_lvars_fv.
   set_solver.
 Qed.
@@ -45,10 +46,10 @@ Qed.
 Lemma lc_lvars_context_tm_support τ e :
   lc_context_ty τ ->
   lc_tm e ->
-  lc_lvars (context_tm_support τ e).
+  lc_lvars (context_ty_lvars τ ∪ tm_lvars e).
 Proof.
   intros Hτ He u Hu.
-  unfold context_tm_support in Hu.
+  cbn [context_ty_lvars context_ty_lvars_at tm_lvars tm_lvars_at value_lvars value_lvars_at] in Hu.
   apply elem_of_union in Hu as [Huτ | Hue].
   - pose proof (cty_lc_at_lvars_bv_empty 0 τ Hτ) as Hbv.
     destruct u as [k|a]; [|exact I].
@@ -98,10 +99,11 @@ Qed.
 Lemma lc_context_tm_support_eq_atoms τ e :
   lc_context_ty τ ->
   lc_tm e ->
-  context_tm_support τ e = lvars_of_atoms (fv_cty τ ∪ fv_tm e).
+  context_ty_lvars τ ∪ tm_lvars e =
+  lvars_of_atoms (fv_cty τ ∪ fv_tm e).
 Proof.
   intros Hτ He.
-  unfold context_tm_support.
+  cbn [context_ty_lvars context_ty_lvars_at tm_lvars tm_lvars_at value_lvars value_lvars_at].
   rewrite (context_ty_lvars_lc_eq_atoms τ Hτ).
   rewrite (tm_lvars_lc_eq_atoms e He).
   unfold lvars_of_atoms.
@@ -139,7 +141,7 @@ Proof.
   rewrite storeA_restrict_dom in Hbad.
   apply elem_of_intersection in Hbad as [_ Hrel].
   apply lvars_fv_elem in Hrel.
-  rewrite relevant_lvars_fv in Hrel.
+  rewrite lvars_fv_union, context_ty_lvars_fv, tm_lvars_fv in Hrel.
   set_solver.
 Qed.
 
@@ -229,7 +231,7 @@ Proof.
   intros Hbasic v Hv.
   pose proof (basic_context_ty_to_lvars _ _ Hbasic) as [Hτ _].
   rewrite lvars_of_atoms_empty in Hτ.
-  unfold relevant_lvars, context_tm_support in Hv.
+  unfold relevant_lvars in Hv.
   cbn [tm_lvars tm_lvars_at value_lvars_at lvar_value_keys] in Hv.
   set_solver.
 Qed.
@@ -279,15 +281,15 @@ Proof.
   - destruct u as [k|y].
     + rewrite lookup_insert_ne by congruence.
       unfold relevant_env, lty_env_restrict_lvars.
-      change (context_tm_support (CTArrow τx τ) (tret v))
+      change (context_ty_lvars (CTArrow τx τ) ∪ tm_lvars (tret v))
         with (relevant_lvars (CTArrow τx τ) (tret v)).
       rewrite storeA_restrict_lookup.
       destruct (decide
         (LVBound k ∈ relevant_lvars (CTArrow τx τ) (tret v))) as [Hin|Hbad].
       { reflexivity. }
       exfalso. apply Hbad.
-      unfold relevant_lvars, context_tm_support in Hu |- *.
-      cbn [relevant_lvars context_tm_support tm_lvars tm_lvars_at value_lvars_at
+      unfold relevant_lvars in Hu |- *.
+      cbn [relevant_lvars tm_lvars tm_lvars_at value_lvars_at
         lvar_value_keys context_ty_lvars context_ty_lvars_at] in Hu |- *.
       better_set_solver.
     + destruct (decide (y = x)) as [->|Hyx].
@@ -296,15 +298,15 @@ Proof.
         exact HΣx.
       * rewrite lookup_insert_ne by congruence.
         unfold relevant_env, lty_env_restrict_lvars.
-        change (context_tm_support (CTArrow τx τ) (tret v))
+        change (context_ty_lvars (CTArrow τx τ) ∪ tm_lvars (tret v))
           with (relevant_lvars (CTArrow τx τ) (tret v)).
         rewrite storeA_restrict_lookup.
         destruct (decide
           (LVFree y ∈ relevant_lvars (CTArrow τx τ) (tret v))) as [Hin|Hbad].
         { reflexivity. }
         exfalso. apply Hbad.
-        unfold relevant_lvars, context_tm_support in Hu |- *.
-        cbn [relevant_lvars context_tm_support tm_lvars tm_lvars_at value_lvars_at
+        unfold relevant_lvars in Hu |- *.
+        cbn [relevant_lvars tm_lvars tm_lvars_at value_lvars_at
           lvar_value_keys context_ty_lvars context_ty_lvars_at] in Hu |- *.
         apply elem_of_union_l.
         apply elem_of_union_l.
@@ -326,7 +328,7 @@ Lemma insert_relevant_env_ret_value_restrict_eq Σ τ v y :
     (relevant_lvars τ (tret (vfvar y))).
 Proof.
   intros Hy.
-  unfold relevant_env, relevant_lvars, context_tm_support, lty_env_restrict_lvars.
+  unfold relevant_env, relevant_lvars, lty_env_restrict_lvars.
   apply storeA_map_eq. intros lv.
   rewrite !storeA_restrict_lookup.
   destruct (decide (lv ∈ context_ty_lvars τ ∪ tm_lvars (tret (vfvar y))))
@@ -339,7 +341,7 @@ Proof.
     destruct (decide (lv ∈ context_ty_lvars τ ∪ tm_lvars (tret v)))
       as [Hvsrc|Hvsrc]; [reflexivity|].
     exfalso.
-    unfold context_tm_support in Hvrel, Hvsrc.
+    cbn [context_ty_lvars context_ty_lvars_at tm_lvars tm_lvars_at value_lvars value_lvars_at] in Hvrel, Hvsrc.
     apply elem_of_union in Hvrel as [Hvτ|Hvy_lvars].
     + apply Hvsrc. apply elem_of_union_l. exact Hvτ.
     + cbn [tm_lvars tm_lvars_at value_lvars_at lvar_value_keys]
@@ -469,7 +471,7 @@ Proof.
         LVFree y ∈ relevant_lvars (cty_open 0 x τ)
           (tapp v1 (vfvar x))).
     {
-      unfold relevant_lvars, context_tm_support.
+      unfold relevant_lvars.
       apply elem_of_union_r. exact Hu.
     }
     rewrite decide_True by exact Hyrel.
@@ -506,7 +508,7 @@ Proof.
         LVFree y ∈ relevant_lvars (cty_open 0 x τ)
           (tapp v1 (vfvar x))).
     {
-      unfold relevant_lvars, context_tm_support.
+      unfold relevant_lvars.
       apply elem_of_union_r. exact Hu.
     }
     rewrite decide_True by exact Hyrel.
@@ -526,7 +528,7 @@ Lemma relevant_lvars_ret_fvar_subset_singleton x τ :
 Proof.
   intros Hbasic v Hv.
   pose proof (basic_context_ty_to_lvars _ _ Hbasic) as [Hτ _].
-  unfold relevant_lvars, context_tm_support in Hv.
+  unfold relevant_lvars in Hv.
   cbn [tm_lvars tm_lvars_at value_lvars_at lvar_value_keys] in Hv.
   unfold lvars_of_atoms in Hτ.
   set_solver.
@@ -539,7 +541,7 @@ Proof.
   intros Hwf v Hv.
   pose proof (wf_context_ty_at_to_lvars_shape 1 ∅ τ Hwf) as [Hτ _].
   rewrite lvars_of_atoms_empty in Hτ.
-  unfold relevant_lvars, context_tm_support in Hv.
+  unfold relevant_lvars in Hv.
   cbn [tm_lvars tm_lvars_at value_lvars_at lvar_value_keys] in Hv.
   set_unfold in Hv.
   destruct Hv as [Hv|Hv].
@@ -731,7 +733,7 @@ Proof.
       unfold relevant_env, lty_env_restrict_lvars.
       apply storeA_restrict_lookup_some_2.
       * apply map_lookup_insert.
-	      * unfold relevant_lvars, context_tm_support.
+	      * unfold relevant_lvars.
 	        cbn [tm_lvars tm_lvars_at value_lvars value_lvars_at].
         set_solver.
     + rewrite lookup_insert_ne in Hv by congruence.
@@ -785,7 +787,7 @@ Lemma relevant_env_lookup_mono_context
 Proof.
   intros Hτ Hlookup.
   unfold relevant_env, lty_env_restrict_lvars,
-    relevant_lvars, context_tm_support in Hlookup |- *.
+    relevant_lvars in Hlookup |- *.
   apply storeA_restrict_lookup_some in Hlookup as [Hv HΣ].
       apply (storeA_restrict_lookup_some_2 _ _ _ _ HΣ). set_solver.
 Qed.
@@ -836,7 +838,7 @@ Lemma relevant_lvars_open k y τ e :
   relevant_lvars (cty_open k y τ) (open_tm k (vfvar y) e).
 Proof.
   intros Hy.
-  unfold relevant_lvars, context_tm_support.
+  unfold relevant_lvars.
   rewrite lvars_open_union.
   rewrite cty_open_vars.
   rewrite tm_lvars_open by exact Hy.
@@ -850,8 +852,12 @@ Lemma relevant_env_open_one k y Σ τ e :
     (cty_open k y τ) (open_tm k (vfvar y) e).
 Proof.
   intros Hy.
-  unfold relevant_env, lty_env_restrict_lvars, lty_env_open_one.
+  unfold relevant_env, lty_env_restrict_lvars.
+  change (context_ty_lvars (cty_open k y τ) ∪
+            tm_lvars (open_tm k (vfvar y) e))
+    with (relevant_lvars (cty_open k y τ) (open_tm k (vfvar y) e)).
   rewrite <- relevant_lvars_open by exact Hy.
+  unfold lty_env_open_one.
   symmetry. apply storeA_restrict_swap.
 Qed.
 
@@ -905,9 +911,9 @@ Proof.
         intros Hbad. apply Hhead.
         eapply lvars_fv_mono; [|exact Hbad].
         apply lvars_open_env_mono.
-	        unfold relevant_lvars, context_tm_support. set_solver.
+	        unfold relevant_lvars. set_solver.
 	      * eapply open_env_fresh_for_lvars_mono; [|exact Hfreshη].
-	        unfold relevant_lvars, context_tm_support. set_solver.
+	        unfold relevant_lvars. set_solver.
 Qed.
 
 Lemma lty_env_restrict_lvars_closed Σ D :
@@ -963,7 +969,7 @@ Lemma basic_typing_lty_env_to_atom_env_relevant Σ τ e T :
   lty_env_to_atom_env (relevant_env Σ τ e) ⊢ₑ e ⋮ T.
 Proof.
   intros Hty.
-  unfold relevant_env, relevant_lvars, context_tm_support.
+  unfold relevant_env, relevant_lvars.
   eapply basic_typing_restrict_lvars_to_atom_env; [|exact Hty].
   set_solver.
 Qed.
@@ -974,7 +980,7 @@ Lemma basic_context_ty_lvars_relevant_env Σ τ e :
 Proof.
   intros [Hvars Hshape]. split; [|exact Hshape].
   intros v Hv.
-  unfold relevant_env, lty_env_restrict_lvars, relevant_lvars, context_tm_support.
+  unfold relevant_env, lty_env_restrict_lvars, relevant_lvars.
   rewrite storeA_restrict_dom.
   apply elem_of_intersection. split; [apply Hvars; exact Hv|set_solver].
 Qed.
@@ -1104,7 +1110,7 @@ Lemma relevant_world_closed_on_term_lvars_eq
 Proof.
   intros Hlvars Hworld Hbasic.
   eapply basic_world_formula_wfworld_closed_on_atoms; [|exact Hworld].
-  unfold relevant_env, relevant_lvars, context_tm_support, lty_env_restrict_lvars.
+  unfold relevant_env, relevant_lvars, lty_env_restrict_lvars.
   rewrite storeA_restrict_dom.
   intros v Hv.
   unfold lvars_of_atoms in Hv.
@@ -1123,7 +1129,7 @@ Proof.
       exact Ha.
     }
     specialize (Hsub _ Ha_lvars).
-    unfold relevant_env, relevant_lvars, context_tm_support,
+    unfold relevant_env, relevant_lvars,
       lty_env_restrict_lvars in Hsub.
     rewrite storeA_restrict_dom in Hsub.
     apply elem_of_intersection in Hsub as [HaΣ _].
@@ -1150,7 +1156,7 @@ Lemma relevant_lvars_insert_fresh x τ e :
   LVFree x ∉ relevant_lvars τ e.
 Proof.
   intros Hxτ Hxe.
-  unfold relevant_lvars, context_tm_support.
+  unfold relevant_lvars.
   pose proof (tm_lvars_free_notin_of_fv x e Hxe).
   set_solver.
 Qed.
@@ -1197,7 +1203,7 @@ Lemma arrow_body_relevant_lvars_subset
   relevant_lvars (CTArrow τx τr) e_src.
 Proof.
   intros Hτ He.
-  unfold relevant_lvars, context_tm_support.
+  unfold relevant_lvars.
   cbn [context_ty_lvars context_ty_lvars_at].
   set_solver.
 Qed.
@@ -1247,7 +1253,7 @@ Lemma wand_arg_relevant_env_agree_insert_core
     (relevant_lvars τx (tret (vfvar y))).
 Proof.
   apply lty_restrict_insert_relevant_eq.
-  unfold relevant_lvars, context_tm_support.
+  unfold relevant_lvars.
   cbn [context_ty_lvars context_ty_lvars_at tm_lvars tm_lvars_at
     value_lvars_at lvar_value_keys].
   set_solver.
@@ -1419,11 +1425,12 @@ Proof.
       rewrite !storeA_rekey_lookup by apply logic_var_shift_from_inj.
       unfold relevant_env, lty_env_restrict_lvars.
       rewrite storeA_restrict_lookup.
-      destruct (decide (LVBound k ∈ context_tm_support
-        (CTWand τx τr) e_src)) as [Hrel|Hrel]; [reflexivity|].
+      destruct (decide (LVBound k ∈
+        context_ty_lvars (CTWand τx τr) ∪ tm_lvars e_src))
+        as [Hrel|Hrel]; [reflexivity|].
       exfalso. apply Hrel.
       subst X.
-      unfold relevant_lvars, context_tm_support in *.
+      unfold relevant_lvars in *.
       cbn [tm_lvars tm_lvars_at value_lvars_at] in *.
       apply elem_of_union in HvX as [Hτopen|Hebody].
       * assert (Hbody : LVBound k ∈ context_ty_lvars_at 1 τr).
@@ -1475,7 +1482,7 @@ Proof.
       }
       subst v.
       subst X.
-      unfold relevant_lvars, context_tm_support in *.
+      unfold relevant_lvars in *.
       cbn [tm_lvars tm_lvars_at value_lvars_at] in *.
       apply elem_of_union in HvX as [Hτopen|Hebody].
       * apply Hyτr.
@@ -1517,11 +1524,12 @@ Proof.
       rewrite !storeA_rekey_lookup by apply logic_var_shift_from_inj.
       unfold relevant_env, lty_env_restrict_lvars.
       rewrite storeA_restrict_lookup.
-      destruct (decide (LVFree z ∈ context_tm_support
-        (CTWand τx τr) e_src)) as [Hrel|Hrel]; [reflexivity|].
+      destruct (decide (LVFree z ∈
+        context_ty_lvars (CTWand τx τr) ∪ tm_lvars e_src))
+        as [Hrel|Hrel]; [reflexivity|].
       exfalso. apply Hrel.
       subst X.
-      unfold relevant_lvars, context_tm_support in *.
+      unfold relevant_lvars in *.
       cbn [tm_lvars tm_lvars_at value_lvars_at] in *.
       apply elem_of_union in HvX as [Hτopen|Hebody].
       * assert (Hbody : LVFree z ∈ context_ty_lvars_at 1 τr).
@@ -1602,7 +1610,7 @@ Proof.
   rewrite lvars_at_depth_typed_lty_env_bind.
   pose proof (lvars_at_depth_relevant_env_subset_relevant
     0 Σ (CTArrow τx τr) e) as Hrel.
-  unfold relevant_lvars, context_tm_support.
+  unfold relevant_lvars.
   rewrite lvars_at_depth_union, context_ty_lvars_depth, tm_lvars_depth.
   rewrite context_ty_lvars_at_shift_under by lia.
   rewrite tm_lvars_at_tret_bound0_under.
@@ -1622,7 +1630,7 @@ Proof.
   pose proof (lvars_at_depth_relevant_env_subset_relevant
     0 Σ (CTArrow τx τr) e) as Hrel.
   pose proof (tm_lvars_at_tapp_shift0_bound0 e 0) as Htapp.
-  unfold relevant_lvars, context_tm_support.
+  unfold relevant_lvars.
   rewrite lvars_at_depth_union, context_ty_lvars_depth, tm_lvars_depth.
   cbn [context_ty_lvars context_ty_lvars_at].
   set_solver.
@@ -1639,7 +1647,7 @@ Proof.
   rewrite lvars_at_depth_typed_lty_env_bind.
   pose proof (lvars_at_depth_relevant_env_subset_relevant
     0 Σ (CTWand τx τr) e) as Hrel.
-  unfold relevant_lvars, context_tm_support.
+  unfold relevant_lvars.
   rewrite lvars_at_depth_union, context_ty_lvars_depth, tm_lvars_depth.
   rewrite context_ty_lvars_at_shift_under by lia.
   rewrite tm_lvars_at_tret_bound0_under.
@@ -1659,7 +1667,7 @@ Proof.
   pose proof (lvars_at_depth_relevant_env_subset_relevant
     0 Σ (CTWand τx τr) e) as Hrel.
   pose proof (tm_lvars_at_tapp_shift0_bound0 e 0) as Htapp.
-  unfold relevant_lvars, context_tm_support.
+  unfold relevant_lvars.
   rewrite lvars_at_depth_union, context_ty_lvars_depth, tm_lvars_depth.
   cbn [context_ty_lvars context_ty_lvars_at].
   set_solver.
@@ -1724,11 +1732,12 @@ Proof.
       rewrite !storeA_rekey_lookup by apply logic_var_shift_from_inj.
       unfold relevant_env, lty_env_restrict_lvars.
       rewrite storeA_restrict_lookup.
-      destruct (decide (LVBound k ∈ context_tm_support (CTWand τx τr) e_src))
+      destruct (decide (LVBound k ∈
+        context_ty_lvars (CTWand τx τr) ∪ tm_lvars e_src))
         as [Hrel|Hrel]; [reflexivity|].
       exfalso. apply Hrel.
       subst X.
-      unfold relevant_lvars, context_tm_support in *.
+      unfold relevant_lvars in *.
       cbn [context_ty_lvars context_ty_lvars_at
         tm_lvars tm_lvars_at value_lvars_at] in *.
       rewrite cty_open_vars in HvX.
@@ -1764,7 +1773,7 @@ Proof.
       }
       subst v.
       subst X.
-      unfold relevant_lvars, context_tm_support in *.
+      unfold relevant_lvars in *.
       cbn [context_ty_lvars context_ty_lvars_at
         tm_lvars tm_lvars_at value_lvars_at] in *.
       rewrite cty_open_vars in HvX.
@@ -1799,11 +1808,12 @@ Proof.
       rewrite !storeA_rekey_lookup by apply logic_var_shift_from_inj.
       unfold relevant_env, lty_env_restrict_lvars.
       rewrite storeA_restrict_lookup.
-      destruct (decide (LVFree z ∈ context_tm_support (CTWand τx τr) e_src))
+      destruct (decide (LVFree z ∈
+        context_ty_lvars (CTWand τx τr) ∪ tm_lvars e_src))
         as [Hrel|Hrel]; [reflexivity|].
       exfalso. apply Hrel.
       subst X.
-      unfold relevant_lvars, context_tm_support in *.
+      unfold relevant_lvars in *.
       cbn [context_ty_lvars context_ty_lvars_at
         tm_lvars tm_lvars_at value_lvars_at] in *.
       rewrite cty_open_vars in HvX.
@@ -1875,11 +1885,11 @@ Proof.
       rewrite !storeA_rekey_lookup by apply logic_var_shift_from_inj.
       unfold relevant_env, lty_env_restrict_lvars.
       rewrite storeA_restrict_lookup.
-      destruct (decide (LVBound k ∈ context_tm_support τsum e_src))
+      destruct (decide (LVBound k ∈ context_ty_lvars τsum ∪ tm_lvars e_src))
         as [Hrel|Hrel]; [reflexivity|].
       exfalso. apply Hrel.
       subst X.
-      unfold relevant_lvars, context_tm_support in *.
+      unfold relevant_lvars in *.
       cbn [tm_lvars tm_lvars_at value_lvars_at] in *.
       rewrite cty_open_vars in HvX.
       unfold context_ty_open_lvars in HvX.
@@ -1913,7 +1923,7 @@ Proof.
       }
       subst v.
       subst X.
-      unfold relevant_lvars, context_tm_support in *.
+      unfold relevant_lvars in *.
       cbn [tm_lvars tm_lvars_at value_lvars_at] in *.
       rewrite cty_open_vars in HvX.
       unfold context_ty_open_lvars in HvX.
@@ -1946,11 +1956,11 @@ Proof.
       rewrite !storeA_rekey_lookup by apply logic_var_shift_from_inj.
       unfold relevant_env, lty_env_restrict_lvars.
       rewrite storeA_restrict_lookup.
-      destruct (decide (LVFree z ∈ context_tm_support τsum e_src))
+      destruct (decide (LVFree z ∈ context_ty_lvars τsum ∪ tm_lvars e_src))
         as [Hrel|Hrel]; [reflexivity|].
       exfalso. apply Hrel.
       subst X.
-      unfold relevant_lvars, context_tm_support in *.
+      unfold relevant_lvars in *.
       cbn [tm_lvars tm_lvars_at value_lvars_at] in *.
       rewrite cty_open_vars in HvX.
       unfold context_ty_open_lvars in HvX.
@@ -2011,7 +2021,7 @@ Notation "'rel[' Σ '|' τ ']' e" :=
    format "rel[ Σ  |  τ ]  e").
 
 Ltac support_lvars_norm :=
-  unfold relevant_lvars, context_tm_support;
+  unfold relevant_lvars;
   type_open_env_syntax_norm;
   cbn [context_ty_lvars context_ty_lvars_at tm_lvars tm_lvars_at
     value_lvars_at lvar_value_keys fv_tm fv_value];
@@ -2031,7 +2041,7 @@ Ltac support_lvars_norm :=
   rewrite ?tm_lvars_at_tret_bound0_under.
 
 Ltac support_lvars_norm_in H :=
-  unfold relevant_lvars, context_tm_support in H;
+  unfold relevant_lvars in H;
   type_open_env_syntax_norm_in H;
   cbn [context_ty_lvars context_ty_lvars_at tm_lvars tm_lvars_at
     value_lvars_at lvar_value_keys fv_tm fv_value] in H;
@@ -2090,14 +2100,14 @@ Ltac lty_env_open_bind_norm_in H :=
   rewrite ?lty_env_open_one_dom in H.
 
 Ltac relevant_env_norm :=
-  unfold relevant_env, lty_env_restrict_lvars, context_tm_support;
+  unfold relevant_env, lty_env_restrict_lvars;
   support_lvars_norm;
   lty_env_open_bind_norm;
   store_normalize;
   rewrite ?storeA_restrict_dom.
 
 Ltac relevant_env_norm_in H :=
-  unfold relevant_env, lty_env_restrict_lvars, context_tm_support in H;
+  unfold relevant_env, lty_env_restrict_lvars in H;
   support_lvars_norm_in H;
   lty_env_open_bind_norm_in H;
   store_normalize;
