ContextTyping/theories/SoundnessLamArrow.v
@@ -633,7 +633,7 @@ Proof.
 	        rewrite <- tm_lvars_fv.
 	        apply (proj2 (lvars_fv_elem _ _)).
 	        exact Hv.
-    + unfold relevant_lvars, context_tm_support. set_solver.
+    + unfold relevant_lvars. set_solver.
 	  - set_solver.
 		  - intros Hzbad.
 		    pose proof (soundness_relevant_env_arrow_value_fresh
@@ -730,7 +730,7 @@ Proof.
 	        rewrite <- tm_lvars_fv.
 	        apply (proj2 (lvars_fv_elem _ _)).
 	        exact Hv.
-    + unfold relevant_lvars, context_tm_support. set_solver.
+    + unfold relevant_lvars. set_solver.
 	  - set_solver.
 		  - intros Hzbad.
 		    pose proof (soundness_relevant_env_wand_value_fresh
